theories/Classes/RelationClasses.v
@@ -20,18 +20,23 @@ Require Import Coq.Program.Basics.
 Require Import Coq.Program.Tactics.
 Require Import Coq.Relations.Relation_Definitions.
 
+(** We will work with computational relations in general, and have specific instances
+   for propositional relations for which we can prove more due to impredicativity of [Prop] *)
+
+Notation crelation A := (A -> A -> Type).
+
 (** We allow to unfold the [relation] definition while doing morphism search. *)
 
-Notation inverse R := (flip (R:relation _) : relation _).
+Notation inverse R := (flip R).
 
-Definition complement {A} (R : relation A) : relation A := fun x y => R x y -> False.
+Definition complement {A} (R : crelation A) := fun x y => R x y -> False.
 
 (** Opaque for proof-search. *)
 Typeclasses Opaque complement.
 
 (** These are convertible. *)
 
-Lemma complement_inverse : forall A (R : relation A), complement (inverse R) = inverse (complement R).
+Lemma complement_inverse : forall A (R : crelation A), complement (inverse R) = inverse (complement R).
 Proof. reflexivity. Qed.
 
 (** We rebind relations in separate classes to be able to overload each proof. *)
@@ -39,21 +44,21 @@ Proof. reflexivity. Qed.
 Set Implicit Arguments.
 Unset Strict Implicit.
 
-Class Reflexive {A} (R : relation A) :=
+Class Reflexive {A} (R : crelation A) :=
   reflexivity : forall x, R x x.
 
-Class Irreflexive {A} (R : relation A) :=
+Class Irreflexive {A} (R : crelation A) :=
   irreflexivity : Reflexive (complement R).
 
 Hint Extern 1 (Reflexive (complement _)) => class_apply @irreflexivity : typeclass_instances.
 
-Class Symmetric {A} (R : relation A) :=
+Class Symmetric {A} (R : crelation A) :=
   symmetry : forall x y, R x y -> R y x.
 
-Class Asymmetric {A} (R : relation A) :=
+Class Asymmetric {A} (R : crelation A) :=
   asymmetry : forall x y, R x y -> R y x -> False.
 
-Class Transitive {A} (R : relation A) :=
+Class Transitive {A} (R : crelation A) :=
   transitivity : forall x y z, R x y -> R y z -> R x z.
 
 Hint Resolve @irreflexivity : ord.
@@ -96,11 +101,11 @@ Hint Extern 3 (Symmetric (flip _)) => class_apply flip_Symmetric : typeclass_ins
 Hint Extern 3 (Asymmetric (flip _)) => class_apply flip_Asymmetric : typeclass_instances.
 Hint Extern 3 (Transitive (flip _)) => class_apply flip_Transitive : typeclass_instances.
 
-Definition Reflexive_complement_Irreflexive `(Reflexive A (R : relation A))
+Definition Reflexive_complement_Irreflexive `(Reflexive A R)
    : Irreflexive (complement R).
 Proof. firstorder. Qed.
 
-Definition complement_Symmetric `(Symmetric A (R : relation A)) : Symmetric (complement R).
+Definition complement_Symmetric `(Symmetric A R) : Symmetric (complement R).
 Proof. firstorder. Qed.
 
 Hint Extern 3 (Symmetric (complement _)) => class_apply complement_Symmetric : typeclass_instances.
@@ -151,23 +156,68 @@ Instance eq_Reflexive {A} : Reflexive (@eq A) := @eq_refl A.
 Instance eq_Symmetric {A} : Symmetric (@eq A) := @eq_sym A.
 Instance eq_Transitive {A} : Transitive (@eq A) := @eq_trans A.
 
+(** The Type arrow. *)
+
+Program Instance arrow_Reflexive : Reflexive arrow.
+Program Instance arrow_Transitive : Transitive arrow.
+
+(** Identity. *)
+
+Program Instance identity_Reflexive : Reflexive (@identity A).
+
+Instance identity_Symmetric : Symmetric (@identity A).
+  reduce. destruct H. reflexivity.
+Defined.
+
+Instance identity_Transitive : Transitive (@identity A).
+  reduce. destruct H. assumption.
+Defined.
+
+(** Type isomorphism. *)
+
+Class Iso (T T' : Type) := { 
+  iso_l : T -> T'; 
+  iso_r : T' -> T;
+  iso_lr : forall x, iso_l (iso_r x) = x ;
+  iso_rl : forall x, iso_r (iso_l x) = x
+}.
+
+Program Instance iso_Reflexive : Reflexive Iso := {
+  reflexivity x := {| iso_l x := x ; iso_r x := x |} }.
+
+Program Instance iso_Symmetric : Symmetric Iso := {
+  symmetry x y isoxy := 
+    {| iso_l := iso_r ; iso_r := iso_l; iso_lr := 
+      iso_rl; iso_rl := iso_lr |} }.
+
+Program Instance iso_Transitive : Transitive Iso := {
+  transitivity A B C isoxy isoyz := 
+    {| iso_l x := iso_l (iso_l x) ;
+      iso_r x := iso_r (iso_r x) |} }.
+
+  Next Obligation.
+  Proof. now do 2 rewrite iso_lr. Defined.
+
+  Next Obligation.
+  Proof. now do 2 rewrite iso_rl. Defined.
+    
 (** Various combinations of reflexivity, symmetry and transitivity. *)
 
 (** A [PreOrder] is both Reflexive and Transitive. *)
 
-Class PreOrder {A} (R : relation A) : Prop := {
+Class PreOrder {A} (R : crelation A) := {
   PreOrder_Reflexive :> Reflexive R | 2 ;
   PreOrder_Transitive :> Transitive R | 2 }.
 
 (** A partial equivalence relation is Symmetric and Transitive. *)
 
-Class PER {A} (R : relation A) : Prop := {
+Class PER {A} (R : crelation A) := {
   PER_Symmetric :> Symmetric R | 3 ;
   PER_Transitive :> Transitive R | 3 }.
 
 (** Equivalence relations. *)
 
-Class Equivalence {A} (R : relation A) : Prop := {
+Class Equivalence {A} (R : crelation A) := {
   Equivalence_Reflexive :> Reflexive R ;
   Equivalence_Symmetric :> Symmetric R ;
   Equivalence_Transitive :> Transitive R }.
@@ -180,7 +230,7 @@ Instance Equivalence_PER `(Equivalence A R) : PER R | 10 :=
 
 (** We can now define antisymmetry w.r.t. an equivalence relation on the carrier. *)
 
-Class Antisymmetric A eqA `{equ : Equivalence A eqA} (R : relation A) :=
+Class Antisymmetric A eqA `{equ : Equivalence A eqA} (R : crelation A) :=
   antisymmetry : forall {x y}, R x y -> R y x -> eqA x y.
 
 Program Definition flip_antiSymmetric `(Antisymmetric A eqA R) :
@@ -196,6 +246,12 @@ Program Instance eq_equivalence : Equivalence (@eq A) | 10.
 (** Logical equivalence [iff] is an equivalence relation. *)
 
 Program Instance iff_equivalence : Equivalence iff.
+
+(** Type identity and isomorphism are equivalences *)
+
+Program Instance identity_equivalence : Equivalence (@identity A) | 10.
+
+Program Instance Iso_equivalence : Equivalence Iso | 9.
 
 (** We now develop a generalization of results on relations for arbitrary predicates.
    The resulting theory can be applied to homogeneous binary relations but also to
@@ -342,16 +398,14 @@ Program Instance predicate_implication_preorder :
     intro. pose (IHl (x x0) (y x0) (z x0)). firstorder.
   Qed.
 
-(** We define the various operations which define the algebra on binary relations,
-   from the general ones. *)
+(** We define the various operations which define the algebra on binary 
+   propositional relations, from the general ones. *)
 
 Definition relation_equivalence {A : Type} : relation (relation A) :=
   @predicate_equivalence (_::_::Tnil).
 
-Class subrelation {A:Type} (R R' : relation A) : Prop :=
-  is_subrelation : @predicate_implication (A::A::Tnil) R R'.
-
-Arguments subrelation {A} R R'.
+Definition relation_implication {A:Type} : relation (relation A) :=
+  @predicate_implication (A::A::Tnil).
 
 Definition relation_conjunction {A} (R : relation A) (R' : relation A) : relation A :=
   @predicate_intersection (A::A::Tnil) R R'.
@@ -367,16 +421,50 @@ Instance relation_equivalence_equivalence (A : Type) :
   Equivalence (@relation_equivalence A).
 Proof. exact (@predicate_equivalence_equivalence (A::A::Tnil)). Qed.
 
-Instance relation_implication_preorder A : PreOrder (@subrelation A).
+Instance relation_implication_preorder A : PreOrder (@relation_implication A).
 Proof. exact (@predicate_implication_preorder (A::A::Tnil)). Qed.
+
+Definition crelation_conjunction {A} (R R' : crelation A) : crelation A :=
+  fun x y => (R x y * R' x y)%type.
+
+Definition crelation_disjunction {A} (R R' : crelation A) : crelation A :=
+  fun x y => (R x y + R' x y)%type.
+
+(** We define the various operations which define the algebra on binary 
+   computational relations directly to avoid inconsistencies. *)
+
+(* Definition crelation_equivalence {A : Type} : crelation (crelation A) := *)
+(*   fun R R' => forall x y, Iso (R x y) (R' x y). *)
+
+Definition crelation_equivalence {A : Type} : crelation (crelation A) :=
+  fun R R' => forall x y, ((R x y -> R' x y) * (R' x y -> R x y)).
+
+Class subrelation {A} (R R' : crelation A) :=
+  is_subrelation : forall x y, R x y -> R' x y.
+
+Arguments subrelation {A} R R'.
+
+Instance crelation_equivalence_equivalence (A : Type) :
+  Equivalence (@crelation_equivalence A).
+Proof. unfold crelation_equivalence. split; red; intros; firstorder.
+  now apply X0, X.
+  now apply X, X0.
+Defined.
+
+Instance crelation_implication_preorder A : PreOrder (@subrelation A).
+Proof. split; red; intros; firstorder. Defined.
+
 
 (** *** Partial Order.
    A partial order is a preorder which is additionally antisymmetric.
    We give an equivalent definition, up-to an equivalence relation
    on the carrier. *)
 
-Class PartialOrder {A} eqA `{equ : Equivalence A eqA} R `{preo : PreOrder A R} :=
+Class PartialOrder {A} (eqA : relation A) `{equ : Equivalence A eqA} (R : relation A) `{preo : PreOrder A R} :=
   partial_order_equivalence : relation_equivalence eqA (relation_conjunction R (inverse R)).
+
+Class CPartialOrder {A} eqA `{equ : Equivalence A eqA} R `{preo : PreOrder A R} :=
+  cpartial_order_equivalence : crelation_equivalence eqA (crelation_conjunction R (inverse R)).
 
 (** The equivalence proof is sufficient for proving that [R] must be a morphism
    for equivalence (see Morphisms).
@@ -385,19 +473,44 @@ Class PartialOrder {A} eqA `{equ : Equivalence A eqA} R `{preo : PreOrder A R} :
 Instance partial_order_antisym `(PartialOrder A eqA R) : ! Antisymmetric A eqA R.
 Proof with auto.
   reduce_goal.
-  pose proof partial_order_equivalence as poe. do 3 red in poe.
-  apply <- poe. firstorder.
-Qed.
+  pose proof partial_order_equivalence as poe. repeat red in poe.
+  specialize (poe x y). apply poe; firstorder.
+Defined.
+
+Instance cpartial_order_antisym `(CPartialOrder A eqA R) : ! Antisymmetric A eqA R.
+Proof with auto.
+  reduce_goal.
+  pose proof cpartial_order_equivalence as poe. repeat red in poe.
+  specialize (poe x y). apply poe; firstorder.
+Defined.
 
 (** The partial order defined by subrelation and relation equivalence. *)
 
 Program Instance subrelation_partial_order :
-  ! PartialOrder (relation A) relation_equivalence subrelation.
+  ! PartialOrder (relation A) relation_equivalence relation_implication.
 
   Next Obligation.
-  Proof.
-    unfold relation_equivalence in *. compute; firstorder.
-  Qed.
+  Proof. unfold relation_equivalence in *; compute; firstorder. Defined.
+
+
+(* Program Definition creleq_conj_subrel A (R R' : crelation A)  *)
+(*   (H : crelation_conjunction subrelation (inverse subrelation) R R') : *)
+(*   crelation_equivalence R R' := *)
+(*   fun x y => {| iso_l := fst H x y ; iso_r := snd H x y |}.  *)
+
+(*   Next Obligation. *)
+(*   Proof. red in H. *)
+(*     destruct H. red in s, s0. simpl.  *)
+(*  destruct H. simpl.  *)
+
+(* Program Instance crelation_partial_order : *)
+(*   ! CPartialOrder (relation A) crelation_equivalence subrelation. *)
+
+(*   Next Obligation. *)
+(*   Proof. *)
+(*     unfold crelation_equivalence, crelation_conjunction. *)
+(*     unfold subrelation. firstorder. *)
+(*   Defined. *)
 
 Typeclasses Opaque arrows predicate_implication predicate_equivalence
   relation_equivalence pointwise_lifting.
@@ -410,11 +523,15 @@ Typeclasses Opaque arrows predicate_implication predicate_equivalence
    relations. This is also done automatically by the [Declare Relation A RA]
    commands. *)
 
-Class RewriteRelation {A : Type} (RA : relation A).
+Class RewriteRelation {A : Type} (RA : crelation A).
 
 Instance: RewriteRelation impl.
 Instance: RewriteRelation iff.
 Instance: RewriteRelation (@relation_equivalence A).
+Instance: RewriteRelation (@crelation_equivalence A).
+Instance: RewriteRelation (@subrelation A).
+Instance: RewriteRelation (@identity A).
+Instance: RewriteRelation Iso.
 
 (** Any [Equivalence] declared in the context is automatically considered
    a rewrite relation. *)
@@ -423,7 +540,7 @@ Instance equivalence_rewrite_relation `(Equivalence A eqA) : RewriteRelation eqA
 
 (** Strict Order *)
 
-Class StrictOrder {A : Type} (R : relation A) : Prop := {
+Class StrictOrder {A : Type} (R : crelation A) := {
   StrictOrder_Irreflexive :> Irreflexive R ;
   StrictOrder_Transitive :> Transitive R
 }.
@@ -436,15 +553,15 @@ Proof. firstorder. Qed.
 Lemma StrictOrder_inverse `(StrictOrder A R) : StrictOrder (inverse R).
 Proof. firstorder. Qed.
 
-(** Same for [PartialOrder]. *)
+(** Same for [PartialOrder], for [relation]s only.  *)
 
-Lemma PreOrder_inverse `(PreOrder A R) : PreOrder (inverse R).
+Lemma PreOrder_inverse `(PreOrder A (R : relation A)) : PreOrder (inverse R).
 Proof. firstorder. Qed.
 
 Hint Extern 3 (StrictOrder (inverse _)) => class_apply StrictOrder_inverse : typeclass_instances.
 Hint Extern 3 (PreOrder (inverse _)) => class_apply PreOrder_inverse : typeclass_instances.
 
-Lemma PartialOrder_inverse `(PartialOrder A eqA R) : PartialOrder eqA (inverse R).
+Lemma PartialOrder_inverse `(PartialOrder A eqA (R : relation A)) : PartialOrder eqA (inverse R).
 Proof. firstorder. Qed.
 
 Hint Extern 3 (PartialOrder (inverse _)) => class_apply PartialOrder_inverse : typeclass_instances.
